proof/refine/ARM/Tcb_R.thy
@@ -1224,9 +1224,9 @@ lemma setMCPriority_valid_objs'[wp]:
    apply (simp add: projectKOs)
   apply (simp add: valid_obj'_def)
   apply (subgoal_tac "tcb_at' t s")
-  apply simp
-  apply (rule valid_tcb'_tcbMCP_update)
-  apply (fastforce  simp: obj_at'_def)+
+   apply simp
+   apply (rule valid_tcb'_tcbMCP_update)
+   apply (fastforce  simp: obj_at'_def)+
   done
 
 crunch sch_act_simple[wp]: setMCPriority sch_act_simple
@@ -1413,9 +1413,9 @@ where
                     | Some (vptr, g'') \<Rightarrow> \<exists>g'''. ipcb' = Some (vptr, g''') \<and> newroot_rel g'' g''') \<and>
         (x = tcbinvocation.ThreadControlCaps t sl' fault_h' time_h' croot' vroot' ipcb'))"
 | "tcbinv_relation (tcb_invocation.ThreadControlSched t sl sc_fault_h prio mcp sc_opt) x
-    = (\<exists>sl' sc_fault_h' sc_opt'.
+    = (\<exists>sl' sc_fault_h'.
          newroot_rel sc_fault_h sc_fault_h'\<and> (sc_fault_h \<noteq> None \<longrightarrow> sl' = cte_map sl) \<and>
-         x = tcbinvocation.ThreadControlSched t sl' sc_fault_h' prio mcp sc_opt')" (* FIXME RT: sc_opt is _opt_opt *)
+         x = tcbinvocation.ThreadControlSched t sl' sc_fault_h' mcp prio sc_opt)"
 | "tcbinv_relation (tcb_invocation.Suspend a) x
     = (x = tcbinvocation.Suspend a)"
 | "tcbinv_relation (tcb_invocation.Resume a) x
@@ -1454,7 +1454,7 @@ where
                 K (valid_option_prio p_auth \<and> valid_option_prio mcp_auth) and
                 (\<lambda>s. case_option True (\<lambda>(pr, auth). mcpriority_tcb_at' ((\<le>) pr) auth s) p_auth) and
                 (\<lambda>s. case_option True (\<lambda>(m, auth). mcpriority_tcb_at' ((\<le>) m) auth s) mcp_auth) and
-                case_option \<top> sc_at' sc_opt)"
+                case_option \<top> (\<lambda>sc_opt'. case_option \<top> (\<lambda>p. sc_at' p and ex_nonz_cap_to' p) sc_opt') sc_opt)"
 | "tcb_inv_wf' (tcbinvocation.ReadRegisters src susp n arch)
              = (tcb_at' src and ex_nonz_cap_to' src)"
 | "tcb_inv_wf' (tcbinvocation.WriteRegisters dest resume values arch)
@@ -1825,383 +1825,920 @@ lemma tc_corres_caps:
                         isValidFaultHandler_def isValidVTableRoot_def | intro conjI)+
   done
 
+lemma get_sc_corres':
+  "corres (\<lambda>sc sc'. sc_relation sc n sc') (sc_obj_at n ptr) (sc_at' ptr)
+          (get_sched_context ptr) (getSchedContext ptr)"
+  apply (rule corres_no_failI)
+   apply wp
+  apply (simp add: get_sched_context_def getSchedContext_def get_object_def
+                   getObject_def bind_assoc)
+  apply (clarsimp simp: in_monad split_def bind_def gets_def get_def return_def)
+  apply (clarsimp simp: assert_def fail_def obj_at_def return_def is_sc_obj_def
+                 split: Structures_A.kernel_object.splits)
+  apply (clarsimp simp: loadObject_default_def in_monad projectKOs
+                        in_magnitude_check objBits_simps' scBits_pos_power2)
+  apply (case_tac ko; clarsimp)
+  apply (clarsimp simp add: state_relation_def pspace_relation_def)
+  apply (drule bspec)
+   apply blast
+  apply clarsimp
+  done
+
+lemma sched_context_unbind_tcb_corres:
+  "corres dc (invs and valid_sched and sc_tcb_sc_at ((\<noteq>) None) scp) invs'
+             (sched_context_unbind_tcb scp) (schedContextUnbindTCB scp)"
+  apply add_sym_refs
+  apply (simp only: sched_context_unbind_tcb_def schedContextUnbindTCB_def)
+  apply (rule corres_stateAssert_assume)
+   apply (rule_tac Q="\<lambda>s. \<exists>n. invs s \<and> valid_sched s \<and>
+                              obj_at (\<lambda>ko. \<exists>sc y. ko = kernel_object.SchedContext sc n \<and>
+                                                  sc_tcb sc = Some y \<and> tcb_at y s) scp s"
+                in stronger_corres_guard_imp)
+     apply (rule corres_underlying_lift_ex1')
+     apply clarsimp
+     apply (rule corres_split')
+        apply (rule corres_guard_imp[OF get_sc_corres'])
+         apply (fastforce simp: obj_at_def is_sc_obj_def valid_obj_def dest: invs_valid_objs)
+        apply (erule conjunct1)
+       apply (rule corres_assert_opt_assume_l)
+       apply (rule corres_assert_assume_r)
+       apply (rule_tac F="sc_tcb sc \<noteq> None" in corres_gen_asm)
+       apply (rule_tac F="\<exists>y. scTCB sca = Some y" in corres_gen_asm2)
+       apply clarsimp
+       apply (rule stronger_corres_guard_imp)
+         apply (rule_tac r'="(=)" in corres_split)
+            apply (clarsimp simp: sc_relation_def)
+            apply (rule_tac r'=dc in corres_split)+
+                        apply (rule_tac f'="scTCB_update Map.empty"
+                                     in update_sc_no_reply_stack_update_ko_at'_corres;
+                               clarsimp simp: sc_relation_def objBits_def objBitsKO_def)
+                       apply (clarsimp simp: set_tcb_obj_ref_thread_set sc_relation_def)
+                       apply (rule threadset_corres; clarsimp simp: tcb_relation_def)
+                      apply (wpsimp simp: set_tcb_obj_ref_def)
+                     apply (wp | rule tcb_release_remove_corres tcbSchedDequeue_corres
+                                      corres_when[OF refl rescheduleRequired_corres] gct_corres)+
+        apply (prop_tac "invs s \<and> (\<exists>y. sc_tcb sc = Some y \<and> tcb_at y s) \<and> weak_valid_sched_action s \<and> sc_at scp s")
+         apply assumption
+        apply (clarsimp simp: invs_def valid_state_def valid_pspace_def sc_relation_def)
+       apply (prop_tac "invs' s' \<and> obj_at' ((=) sca) scp s'")
+        apply assumption
+       apply clarsimp
+       apply (frule tcb_at_cross[rotated 3]; fastforce simp: obj_at'_def sc_relation_def)
+      apply wp
+      apply (fastforce dest: invs_valid_objs simp: valid_obj_def obj_at_def is_sc_obj_def)
+     apply wp
+     apply clarsimp
+     apply (prop_tac "invs' s \<and> obj_at' (\<lambda>sc. scTCB sc \<noteq> None) scp s")
+      apply assumption
+     apply (clarsimp simp: obj_at'_def)
+    apply (clarsimp simp: obj_at_def sc_at_ppred_def neq_commute)
+    apply (drule invs_valid_objs)
+    apply (erule (1) valid_objsE)
+    apply (clarsimp simp: valid_obj_def valid_sched_context_def valid_bound_obj_def obj_at_def)
+   apply (subgoal_tac "sc_at_pred (\<lambda>sc. sc_tcb sc \<noteq> None) scp s")
+    apply clarsimp
+    apply (subgoal_tac "obj_at' (\<lambda>sc. \<exists>y. scTCB sc = Some y) scp s'")
+     apply (clarsimp simp: sc_at_pred_def obj_at_def obj_at'_def)
+    apply (prop_tac "sc_at scp s")
+     apply (clarsimp simp: sc_at_pred_def obj_at_def obj_at'_def is_sc_obj_def)
+     apply (fastforce dest: invs_valid_objs simp: valid_obj_def)
+    apply (drule sc_at_cross[rotated 3], fastforce, fastforce, fastforce)
+    apply (clarsimp simp: sc_at_pred_def obj_at_def obj_at'_def projectKO_eq)
+    apply (drule state_relation_pspace_relation)
+    apply (drule (1) pspace_relation_absD)
+    apply (clarsimp simp: sc_relation_def split: if_splits kernel_object.splits)
+   apply (clarsimp simp: obj_at_def sc_at_ppred_def neq_commute)
+  apply (clarsimp simp: sym_refs_asrt_def)
+  done
+
+lemma get_tcb_sc_corres:
+  "corres (\<lambda>x y. \<exists>n. sc_relation x n y)
+          (\<lambda>s. bound_sc_tcb_at (\<lambda>sc. \<exists>y. sc = Some y \<and> sc_at y s) t s)
+          (\<lambda>s. bound_sc_tcb_at' (\<lambda>sc. \<exists>y. sc = Some y \<and> sc_at' y s) t s)
+          (get_tcb_sc t) (getTCBSc t)"
+  unfolding get_tcb_sc_def getTCBSc_def
+  apply (rule corres_guard_imp)
+    apply (rule_tac r'="(=)" in corres_split)
+       apply clarsimp
+       apply (rule corres_assert_opt_assume_l)
+       apply (rule corres_assert_assume_r)
+       apply (rule get_sc_corres)
+      apply (clarsimp simp: get_tcb_obj_ref_def)
+      apply (rule threadget_corres, simp add: tcb_relation_def)
+     apply (clarsimp simp: get_tcb_obj_ref_def)
+     apply (wp thread_get_wp)
+    apply (wp threadGet_wp)
+   apply clarsimp
+   apply (fastforce simp: pred_tcb_at_def obj_at_def is_tcb_def)
+  apply (clarsimp simp: pred_tcb_at'_def obj_at'_def)
+  done
+
+lemma r_time_cross:
+  "\<lbrakk> valid_sched_context sc s; valid_sched_context' sc' s';
+     sc_relation sc n sc'; sc_active sc; sc_refills sc \<noteq> [] \<rbrakk>
+     \<Longrightarrow> r_time (refill_hd sc) = rTime (refillHd sc')"
+  by (clarsimp simp: valid_sched_context_def valid_sched_context'_def
+                     refillHd_def refills_map_def refill_map_def wrap_slice_def
+                     sc_relation_def active_sc_def hd_map hd_drop_conv_nth)
+
+lemma r_amount_cross:
+  "\<lbrakk> valid_sched_context sc s; valid_sched_context' sc' s';
+     sc_relation sc n sc'; sc_active sc; sc_refills sc \<noteq> [] \<rbrakk>
+     \<Longrightarrow> r_amount (refill_hd sc) = rAmount (scRefills sc' ! scRefillHead sc')"
+  by (clarsimp simp: valid_sched_context_def valid_sched_context'_def
+                     refillHd_def refills_map_def refill_map_def wrap_slice_def
+                     sc_relation_def active_sc_def hd_map hd_drop_conv_nth)
+
+lemma get_sc_time_corres:
+  "corres (=) (\<lambda>s. invs s \<and> bound_sc_tcb_at (\<lambda>sc. \<exists>y. sc = Some y \<and> valid_refills y s) x s) invs'
+              (get_sc_time x) (getScTime x)"
+  apply (simp only: get_sc_time_def getScTime_def)
+  apply (rule stronger_corres_guard_imp)
+    apply (rule corres_split[OF _ get_tcb_sc_corres])
+      apply clarsimp
+      apply (prop_tac "valid_sched_context sc s \<and>
+                       (\<exists>tcb y. ko_at (TCB tcb) x s \<and> tcb_sched_context tcb = Some y \<and>
+                                valid_refills y s \<and> sc_at_pred ((=) sc) y s)", assumption)
+      apply (clarsimp simp: obj_at_def sc_at_pred_n_def)
+      apply (rule_tac s=s and s'=s' in r_time_cross; assumption?)
+       apply (auto simp: pred_map_def cfg_valid_refills_def rr_valid_refills_def active_sc_def
+                         sp_valid_refills_def sc_refill_cfgs_of_scs_def map_project_def
+                         scs_of_kh_def opt_map_def sc_of_def MIN_REFILLS_def sc_of_def
+                  split: if_splits)[2]
+     apply (wpsimp wp: thread_get_wp simp: get_tcb_sc_def get_tcb_obj_ref_def)
+    apply (wpsimp wp: threadGet_wp simp: getTCBSc_def)
+   apply (clarsimp simp: sc_at_pred_n_def pred_tcb_at_def obj_at_def)
+   apply (drule invs_valid_objs)
+   apply (erule valid_objsE[rotated]; fastforce simp: valid_obj_def valid_tcb_def obj_at_def)
+  apply clarsimp
+  apply (rule context_conjI)
+   apply (prop_tac "tcb_at' x s'")
+    apply (rule tcb_at_cross; fastforce simp: pred_tcb_at_def obj_at_def is_tcb_def)
+   apply (clarsimp simp: pred_tcb_at_def pred_tcb_at'_def obj_at_def state_relation_def)
+   apply (drule (1) pspace_relation_absD)
+   apply (clarsimp simp: other_obj_relation_def)
+   apply (clarsimp split: kernel_object.splits)
+   apply (fastforce simp: valid_obj'_def valid_tcb'_def valid_bound_obj'_def
+                          obj_at'_def projectKOs tcb_relation_def
+                    dest: invs_valid_objs' split: option.splits)+
+  done
+
+lemma tcb_release_enqueue_corres:
+  "corres dc (\<lambda>s. invs s \<and> valid_release_q s \<and> active_sc_valid_refills s \<and>
+                  bound_sc_tcb_at (\<lambda>sc. \<exists>y. sc = Some y \<and> valid_refills y s) t s) invs'
+             (tcb_release_enqueue t) (tcbReleaseEnqueue t)"
+  apply (clarsimp simp: tcb_release_enqueue_def tcbReleaseEnqueue_def setReleaseQueue_def)
+  apply (rule stronger_corres_guard_imp)
+    apply (rule_tac r'="(=)" in corres_split)
+       apply (rule_tac r'="(=)" in corres_split)
+          apply (rule_tac r'="(=)" in corres_split)
+             apply (rule corres_split)
+                apply (rule corres_add_noop_lhs2)
+                apply (rule corres_split)
+                   apply (rule threadSet_corres_noop; clarsimp simp: tcb_relation_def)
+                  apply (rule corres_modify)
+                  apply (clarsimp simp: state_relation_def release_queue_relation_def swp_def)
+                 apply wp
+                apply wp
+               apply clarsimp
+               apply (rule corres_when, simp)
+               apply (rule reprogram_timer_corres)
+              apply (rule hoare_strengthen_post[OF hoare_post_taut], simp)
+             apply (rule_tac Q="\<lambda>_. P and P" for P in hoare_triv)
+             apply wpsimp
+            apply (rule_tac r'="(=)" and S="(=)" in corres_mapM_list_all2; clarsimp)
+               apply (clarsimp simp: list.rel_eq)
+               apply wpfix
+               apply (rule_tac P="\<lambda>s. invs s \<and>
+                                      (\<forall>x \<in> set (y#ys). bound_sc_tcb_at (\<lambda>sc. \<exists>y. sc = Some y \<and>
+                                                                                   valid_refills y s) x s)"
+                            in corres_guard1_imp)
+                apply (rule get_sc_time_corres, simp)
+              apply wpsimp
+             apply (wpsimp simp: getScTime_def getTCBSc_def wp: hoare_drop_imps)
+            apply (clarsimp simp: list.rel_eq)
+           apply (wpsimp wp: mapM_get_sc_time_wp)
+          apply (wpsimp wp: mapM_wp_lift threadGet_wp
+                      simp: getScTime_def getTCBSc_def list_all2_eq_iff_map_eq_map obj_at'_def)
+         apply (rule release_queue_corres)
+        apply wp
+       apply (wpsimp simp: getReleaseQueue_def)
+      apply (rule get_sc_time_corres)
+     apply wp
+    apply (wpsimp wp: threadGet_wp simp: getScTime_def getTCBSc_def)
+   apply (fastforce simp: active_implies_valid_refills_tcb_at valid_sched_def valid_release_q_def)
+  apply (clarsimp simp: obj_at'_def)
+  done
+
+lemma postpone_corres:
+  "corres dc (\<lambda>s. invs s \<and> valid_release_q s \<and> active_sc_valid_refills s
+                         \<and> (\<exists>sc n. ko_at (kernel_object.SchedContext sc n) ptr s
+                         \<and> (\<exists>tcb. sc_tcb sc = Some tcb \<and> not_queued tcb s
+                         \<and> bound_sc_tcb_at (\<lambda>sc. \<exists>y. sc = Some y \<and> valid_refills y s) tcb s))) invs'
+             (SchedContext_A.postpone ptr) (postpone ptr)"
+  apply (rule stronger_corres_guard_imp)
+    apply (clarsimp simp: SchedContext_A.postpone_def postpone_def get_sc_obj_ref_def)
+    apply (rule_tac r'="\<lambda>sc sca. \<exists>n. sc_relation sc n sca" in corres_split)
+       apply (rule corres_assert_opt_assume_l)
+       apply (rule corres_split)
+          apply (rule corres_split)
+             apply (rule reprogram_timer_corres)
+            apply (clarsimp simp: sc_relation_def)
+            apply (rule tcb_release_enqueue_corres)
+           apply wp
+          apply wp
+         apply (clarsimp simp: sc_relation_def)
+         apply (rule_tac P="tcb_at (the (sc_tcb rv))" in corres_guard1_imp)
+          apply (rule tcbSchedDequeue_corres)
+         apply clarsimp
+        apply (wp tcb_sched_dequeue_not_queued_inv)
+        apply (subgoal_tac "scTCB rv' = sc_tcb rv")
+         apply clarsimp
+         apply assumption
+        apply (clarsimp simp: sc_relation_def)
+       apply wpsimp
+      apply (rule get_sc_corres)
+     apply wp
+    apply wp
+   apply (fastforce simp: valid_obj_def pred_tcb_at_def obj_at_def is_tcb_def is_sc_obj_def
+                    dest: invs_valid_objs)
+  apply clarsimp
+  apply (intro conjI impI allI)
+    apply (rule sc_at_cross)
+       apply fastforce
+      apply fastforce
+     apply fastforce
+    apply (fastforce dest: invs_valid_objs simp: obj_at_def is_sc_obj_def valid_obj_def)
+   apply (clarsimp simp: state_relation_def obj_at_def)
+   apply (frule (1) pspace_relation_absD[rotated])
+   apply (clarsimp split: if_splits)
+   apply (case_tac z; clarsimp)
+   apply (rule tcb_at_cross)
+      apply fastforce
+     apply fastforce
+    apply fastforce
+   apply (drule invs_valid_objs)
+   apply (erule (1) valid_objsE)
+   apply (simp only: sc_relation_def eq_commute[where a="Some P" for P] Some_to_the)
+   apply (clarsimp simp: obj_at'_def projectKO_eq projectKO_sc)
+  apply clarsimp
+  done
+
+lemma get_sc_refill_ready_def':
+  "get_sc_refill_ready sc_ptr = do cur_time \<leftarrow> gets cur_time;
+                                   sc \<leftarrow> get_sched_context sc_ptr;
+                                   return $ sc_refill_ready cur_time sc
+                                od"
+  apply (rule ext)
+  apply (auto simp: get_sc_refill_ready_def get_sched_context_def get_object_def
+                    gets_def get_def bind_def assert_def return_def fail_def
+             split: Structures_A.kernel_object.splits)
+  done
+
+lemma get_sc_refill_ready_corres:
+  "corres (=) (invs and sc_at_pred sc_active ptr and active_sc_valid_refills) invs'
+              (get_sc_refill_ready ptr) (refillReady ptr)"
+  apply (simp only: get_sc_refill_ready_def' refillReady_def getCurTime_def)
+  apply (rule stronger_corres_guard_imp)
+    apply (rule_tac r'="(=)" in corres_split)
+       apply (rule_tac R="\<lambda>rv s. invs s \<and> active_sc_valid_refills s \<and>
+                                 sc_at_pred (\<lambda>sc. sc = rv \<and> sc_active sc) ptr s"
+                   and R'="\<lambda>rv' s. invs' s \<and> ko_at' rv' ptr s"
+                   and r'="\<lambda>sc sc'. \<exists>n. sc_relation sc n sc'" in corres_split)
+          apply (clarsimp simp: refill_ready_def)
+          apply (subgoal_tac "r_time (refill_hd rva) = rTime (refillHd rv'a)")
+           apply (clarsimp simp: kernelWCETTicks_def)
+          apply (rule_tac s=s in r_time_cross)
+              apply (fastforce simp: valid_obj_def obj_at_def sc_at_pred_def valid_obj'_def
+                                     obj_at'_def projectKOs active_sc_def MIN_REFILLS_def
+                                     pred_map_def cfg_valid_refills_def rr_valid_refills_def
+                                     sp_valid_refills_def sc_refill_cfgs_of_scs_def map_project_def
+                                     scs_of_kh_def opt_map_def sc_of_def active_sc_valid_refills_def
+                               dest: invs_valid_objs invs_valid_objs' split: option.splits)+
+         apply (rule get_sc_corres)
+        apply (wpsimp simp: state_relation_def)+
+   apply (fastforce simp: valid_obj_def obj_at_def sc_at_pred_def is_sc_obj_def
+                    dest: invs_valid_objs intro: sc_at_cross)+
+  done
+
+lemma get_sc_refill_sufficient_corres:
+  "corres (=) (invs and sc_at_pred sc_active ptr and active_sc_valid_refills) invs'
+              (get_sc_refill_sufficient ptr 0) (refillSufficient ptr 0)"
+  apply (simp only: get_sc_refill_sufficient_def refillSufficient_def getRefills_def)
+  apply (rule stronger_corres_guard_imp)
+    apply (rule corres_symb_exec_r)
+       apply (rule_tac R="\<lambda>rv s. invs s \<and> active_sc_valid_refills s \<and>
+                                 sc_at_pred (\<lambda>sc. sc = rv \<and> sc_active sc) ptr s"
+                   and R'= "\<lambda>rv' s. invs' s \<and> ko_at' rv' ptr s \<and> refills = scRefills rv'"
+                   and r'="\<lambda>sc sc'. \<exists>n. sc_relation sc n sc'" in corres_split)
+          apply (clarsimp simp: refill_sufficient_def sufficientRefills_def
+                                refill_capacity_def refillsCapacity_def)
+          apply (subgoal_tac "r_amount (refill_hd rv) = rAmount (scRefills rv' ! scRefillHead rv')")
+           apply (clarsimp simp: MIN_BUDGET_def minBudget_def
+                                 kernelWCET_ticks_def kernelWCETTicks_def)
+          apply (rule_tac s=s in r_amount_cross)
+              apply (fastforce simp: valid_obj_def obj_at_def sc_at_pred_def valid_obj'_def
+                                     obj_at'_def projectKOs active_sc_def MIN_REFILLS_def
+                                     pred_map_def cfg_valid_refills_def rr_valid_refills_def
+                                     sp_valid_refills_def sc_refill_cfgs_of_scs_def map_project_def
+                                     scs_of_kh_def opt_map_def sc_of_def active_sc_valid_refills_def
+                               dest: invs_valid_objs invs_valid_objs' split: option.splits)+
+         apply (rule get_sc_corres)
+        apply wp
+       apply wp
+      apply (rule hoare_weaken_pre, wp)
+      apply (erule conjunct1)
+     apply wpsimp
+    apply wpsimp
+    apply assumption
+   apply (fastforce simp: valid_obj_def obj_at_def sc_at_pred_def is_sc_obj_def obj_at'_def
+                    dest: invs_valid_objs intro: sc_at_cross)+
+  done
+
+lemma sched_context_resume_corres:
+  "corres dc (\<lambda>s. invs s \<and>  valid_ready_qs s \<and> valid_release_q s \<and> active_sc_valid_refills s \<and>
+                  sc_tcb_sc_at (\<lambda>tcb. tcb = Some t \<and> bound_sc_tcb_at (\<lambda>sc. sc = Some ptr) t s) ptr s)
+             invs'
+             (sched_context_resume ptr) (schedContextResume ptr)"
+  apply (simp only: sched_context_resume_def schedContextResume_def)
+  apply (rule stronger_corres_guard_imp)
+    apply clarsimp
+    apply (rule_tac r'="\<lambda>sc sca. \<exists>n. sc_relation sc n sca" in corres_split)
+       apply (rename_tac sc sca)
+       apply (rule corres_assert_opt_assume_l)
+       apply (rule corres_assert_assume_r)
+       apply (rule_tac r'="(=)" in corres_split)
+          apply (rule corres_when)
+           apply clarsimp
+          apply (rule corres_symb_exec_l)
+             apply (rule_tac F="runnable ts \<and> sc_active sc" in corres_gen_asm)
+             apply (rule_tac r'="(=)" in corres_split)
+                apply (rule_tac r'="(=)" in corres_split)
+                   apply (rule corres_when)
+                    apply clarsimp
+                   apply (rule corres_symb_exec_l)
+                      apply (rule corres_symb_exec_l)
+                         apply (rule corres_symb_exec_l)
+                            apply (rule corres_assert_assume_l)
+                            apply (rule postpone_corres)
+                           apply (wpsimp simp: get_tcb_queue_def)
+                          apply wp
+                         apply (clarsimp simp: no_fail_def get_tcb_queue_def gets_def get_def)
+                        prefer 2
+                        apply (wp thread_get_wp)
+                       apply (wp thread_get_exs_valid)
+                        apply (clarsimp simp: obj_at_def is_tcb_def)
+                       apply clarsimp
+                      apply (clarsimp simp: no_fail_def obj_at_def thread_get_def
+                                            gets_the_def get_tcb_def gets_def get_def
+                                            assert_opt_def bind_def return_def)
+                     prefer 2
+                     apply (wp thread_get_wp)
+                    apply (wp thread_get_exs_valid)
+                     apply (clarsimp simp: obj_at_def is_tcb_def)
+                    apply clarsimp
+                   apply (clarsimp simp: no_fail_def obj_at_def thread_get_def
+                                         gets_the_def get_tcb_def gets_def get_def
+                                         assert_opt_def bind_def return_def)
+                  apply (rule get_sc_refill_sufficient_corres)
+                 apply wp
+                apply (wpsimp simp: refillSufficient_def getRefills_def)
+               apply (rule get_sc_refill_ready_corres)
+              apply wp
+             apply (wpsimp simp: refillReady_def getCurTime_def)
+            apply (rule thread_get_exs_valid)
+            apply (erule conjunct1)
+           apply (wp thread_get_wp)
+           apply (clarsimp cong: conj_cong)
+           apply assumption
+          apply clarsimp
+          apply (rule no_fail_pre)
+           apply (wpsimp simp: thread_get_def)
+          apply (clarsimp simp: tcb_at_def)
+         apply (clarsimp simp: sc_relation_def)
+         apply (rule corres_guard_imp)
+           apply (rule isSchedulable_corres)
+          apply (prop_tac "(valid_objs and tcb_at (the (sc_tcb sc))
+                                       and pspace_aligned and pspace_distinct) s")
+           apply assumption
+          apply clarsimp
+         apply assumption
+        apply (wp is_schedulable_wp)
+       apply (wp isSchedulable_wp)
+      apply (rule get_sc_corres)
+     apply wp
+    apply wp
+   apply (clarsimp simp: sc_at_ppred_def obj_at_def is_sc_obj_def bound_sc_tcb_at_def is_tcb_def)
+   apply (intro conjI impI; clarsimp simp: invs_def valid_state_def)
+         apply (fastforce simp: valid_pspace_def valid_obj_def)
+        apply (fastforce simp: is_schedulable_bool_def get_tcb_def is_sc_active_def)
+       apply (clarsimp simp: in_ready_q_def)
+       apply (fastforce simp: valid_ready_qs_2_def valid_ready_queued_thread_2_def
+                              pred_map2'_def sc_refill_cfgs_of_scs_def tcb_scps_of_tcbs_def
+                              map_project_def scs_of_kh_def sc_of_def tcbs_of_kh_def tcb_of_def)
+      apply (fastforce elim: active_sc_valid_refillsE[rotated]
+                       simp: is_active_sc_def sc_refill_max_sc_at_def active_sc_at_def)
+     apply (fastforce simp: valid_ready_qs_2_def valid_ready_queued_thread_2_def
+                            pred_map2'_def sc_refill_cfgs_of_scs_def tcb_scps_of_tcbs_def
+                            map_project_def scs_of_kh_def sc_of_def tcbs_of_kh_def tcb_of_def)
+    apply (clarsimp simp: is_schedulable_bool_def get_tcb_def)
+   apply (clarsimp simp: is_schedulable_bool_def get_tcb_def is_sc_active_def split: option.splits)
+  apply (clarsimp simp: invs'_def valid_state'_def valid_pspace'_def)
+  apply (intro conjI impI allI)
+    apply (fastforce simp: sc_at_ppred_def obj_at_def is_sc_obj_def valid_obj_def
+                     dest: invs_valid_objs intro!: sc_at_cross)
+   apply clarsimp
+  apply (clarsimp simp: state_relation_def obj_at_def sc_at_ppred_def)
+  apply (drule (1) pspace_relation_absD)
+  apply (clarsimp split: if_splits)
+  apply (case_tac z; clarsimp simp: sc_relation_def)
+  apply (simp only: sc_relation_def eq_commute[where a="Some P" for P])
+  apply (clarsimp simp: obj_at'_def projectKO_eq projectKO_sc)
+  done
+
+abbreviation all_invs'_but_valid_release_queue where
+  "all_invs'_but_valid_release_queue \<equiv>
+   \<lambda>s. valid_pspace' s \<and> sch_act_wf (ksSchedulerAction s) s
+                       \<and> valid_queues s
+                       \<and> sym_refs (list_refs_of_replies' s)
+                       \<and> if_live_then_nonz_cap' s \<and> if_unsafe_then_cap' s
+                       \<and> valid_idle' s
+                       \<and> valid_global_refs' s \<and> valid_arch_state' s
+                       \<and> valid_irq_node' (irq_node' s) s
+                       \<and> valid_irq_handlers' s
+                       \<and> valid_irq_states' s
+                       \<and> valid_machine_state' s
+                       \<and> irqs_masked' s
+                       \<and> valid_queues' s
+                       \<and> ct_not_inQ s
+                       \<and> ct_idle_or_in_cur_domain' s
+                       \<and> valid_pde_mappings' s
+                       \<and> pspace_domain_valid s
+                       \<and> ksCurDomain s \<le> maxDomain
+                       \<and> valid_dom_schedule' s
+                       \<and> untyped_ranges_zero' s
+                       \<and> cur_tcb' s"
+
+lemma threadSet_tcbInReleaseQueue_invs':
+  "\<lbrace>\<lambda>s. all_invs'_but_valid_release_queue s \<and>
+        (\<forall>tcb. ko_at' tcb tptr s \<longrightarrow>
+                valid_release_queue_iff
+                  (s\<lparr>ksPSpace := ksPSpace s(tptr \<mapsto> KOTCB (tcbInReleaseQueue_update (\<lambda>_. v) tcb))\<rparr>))\<rbrace>
+   threadSet (tcbInReleaseQueue_update (\<lambda>_. v)) tptr
+   \<lbrace>\<lambda>_. invs'\<rbrace>"
+  apply (clarsimp simp add: invs'_def valid_state'_def split del: if_split)
+  apply (wp threadSet_valid_pspace'T threadSet_sch_actT_P[where P=False, simplified]
+           threadSet_iflive'T threadSet_ifunsafe'T threadSet_idle'T threadSet_not_inQ
+           valid_irq_node_lift valid_irq_handlers_lift'' threadSet_ct_idle_or_in_cur_domain'
+           threadSet_cur untyped_ranges_zero_lift threadSet_valid_queues threadSet_valid_queues'
+         | rule refl threadSet_wp [THEN hoare_vcg_conj_lift]
+         | clarsimp simp: tcb_cte_cases_def cteCaps_of_def)+
+  apply (fastforce simp: obj_at'_def projectKO_eq projectKO_tcb objBitsKO_def inQ_def comp_def )
+  done
+
+lemma getScTime_wp:
+  "\<lbrace>\<lambda>s. \<forall>rt. (\<forall>tcb p sc. (ko_at' tcb t s \<and> tcbSchedContext tcb = Some p \<and> ko_at' sc p s
+                                                          \<longrightarrow> rTime (refillHd sc) = rt)) \<longrightarrow> Q rt s\<rbrace>
+   getScTime t \<lbrace>Q\<rbrace>"
+  by (wpsimp wp: threadGet_wp simp: getScTime_def getTCBSc_def obj_at'_def)
+
+schematic_goal mapM_getScTime_wp:
+  "\<lbrace>?P\<rbrace> mapM getScTime ts \<lbrace>Q\<rbrace>"
+  by (wp mapM_wp_lift getScTime_wp)
+
+lemma ct_not_inQ_ksReleaseQueue_upd[simp]:
+  "ct_not_inQ (s\<lparr>ksReleaseQueue := v\<rparr>) = ct_not_inQ s"
+  by (simp add: ct_not_inQ_def)
+
+lemma valid_irq_node'_ksReleaseQueue_upd[simp]:
+  "valid_irq_node' (irq_node' s) (s\<lparr>ksReleaseQueue := v\<rparr>) = valid_irq_node' (irq_node' s) s"
+  by (simp add: valid_irq_node'_def)
+
+lemma cur_tcb'_ksReleaseQueue_upd[simp]:
+  "cur_tcb' (s\<lparr>ksReleaseQueue := v\<rparr>) = cur_tcb' s"
+  by (simp add: cur_tcb'_def)
+
+lemma valid_queues_ksReleaseQueue_upd[simp]:
+  "valid_queues (s\<lparr>ksReleaseQueue := v\<rparr>) = valid_queues s"
+  by (simp add: valid_queues_def valid_queues_no_bitmap_def valid_bitmapQ_def
+                bitmapQ_def bitmapQ_no_L1_orphans_def bitmapQ_no_L2_orphans_def)
+
+lemma valid_queues'_ksReleaseQueue_upd[simp]:
+  "valid_queues' (s\<lparr>ksReleaseQueue := v\<rparr>) = valid_queues' s"
+  by (simp add: valid_queues'_def)
+
+lemma ksReleaseQueue_ksReprogramTimer_update:
+  "ksReleaseQueue_update (\<lambda>_. fv) (ksReprogramTimer_update (\<lambda>_. gv) s) =
+   ksReprogramTimer_update (\<lambda>_. gv) (ksReleaseQueue_update (\<lambda>_. fv) s)"
+  by simp
+
+lemma ksPSpace_ksReprogramTimer_update:
+  "ksPSpace_update (\<lambda>_. fv) (ksReprogramTimer_update (\<lambda>_. gv) s) =
+   ksReprogramTimer_update (\<lambda>_. gv) (ksPSpace_update (\<lambda>_. fv) s)"
+  by simp
+
+lemma tcbReleaseEnqueue_invs'[wp]:
+  "tcbReleaseEnqueue tcb \<lbrace>invs'\<rbrace>"
+  apply (clarsimp simp: getScTime_def getTCBSc_def tcbReleaseEnqueue_def
+                        getReleaseQueue_def setReleaseQueue_def setReprogramTimer_def)
+  apply (wpsimp wp: threadSet_tcbInReleaseQueue_invs')
+     apply (clarsimp simp: ksReleaseQueue_ksReprogramTimer_update
+                           ksPSpace_ksReprogramTimer_update if_cancel_eq_True)
+     apply (wpsimp wp: mapM_getScTime_wp threadGet_wp)+
+  apply (clarsimp simp: invs'_def valid_state'_def comp_def obj_at'_def)
+  apply (rule conjI)
+   apply (clarsimp simp: valid_release_queue_def obj_at'_def projectKO_eq projectKO_tcb objBitsKO_def)
+   apply (intro conjI impI; clarsimp)
+       apply (auto split: if_splits elim: ps_clear_domE)[3]
+    apply (drule_tac x=a in spec, drule mp)
+     apply (rule_tac ys=rvs in tup_in_fst_image_set_zipD)
+     apply (clarsimp simp: Set.image_def)
+     apply (rule_tac x="(a,b)" in bexI)
+      apply (auto split: if_splits elim: ps_clear_domE)[3]
+   apply (drule_tac x=a in spec, drule mp)
+    apply (rule_tac ys=rvs in tup_in_fst_image_set_zipD)
+    apply (clarsimp simp: Set.image_def)
+    apply (rule_tac x="(a,b)" in bexI)
+     apply (auto split: if_splits elim: ps_clear_domE)[3]
+  apply (clarsimp simp: valid_release_queue'_def)
+  apply (erule_tac x=t in allE)
+  apply (drule mp)
+   apply (fastforce simp: obj_at'_def projectKO_eq projectKO_tcb objBitsKO_def inQ_def
+                    elim: ps_clear_domE split: if_splits)
+  apply (clarsimp simp: image_def in_set_conv_decomp zip_append1)
+  apply (rule_tac x="hd (drop (length ys) rvs)" in exI)
+  apply (case_tac "drop (length ys) rvs"; fastforce dest: list_all2_lengthD)
+  done
+
+crunches postpone, schedContextResume
+  for invs': invs'
+  (wp: crunch_wps)
+
+lemma threadSet_mdb':
+  "\<lbrace>valid_mdb' and obj_at' (\<lambda>t. \<forall>(getF, setF) \<in> ran tcb_cte_cases. getF t = getF (f t)) t\<rbrace>
+   threadSet f t
+   \<lbrace>\<lambda>rv. valid_mdb'\<rbrace>"
+  by (wpsimp wp: setObject_tcb_mdb' getTCB_wp simp: threadSet_def obj_at'_def)
+
+lemma sched_context_resume_weak_valid_sched_action:
+  "\<lbrace>\<lambda>s. weak_valid_sched_action s \<and>
+        (\<forall>ya. sc_tcb_sc_at ((=) (Some ya)) scp s \<longrightarrow> scheduler_act_not ya s)\<rbrace>
+   sched_context_resume scp
+   \<lbrace>\<lambda>_. weak_valid_sched_action\<rbrace>"
+  unfolding sched_context_resume_def
+  by (wpsimp wp: postpone_weak_valid_sched_action thread_get_wp' is_schedulable_wp')
+
+crunches sched_context_resume
+  for sc_at_ppred[wp]: "sc_at_ppred n P ptr"
+  (wp: crunch_wps)
+
+lemma sched_context_bind_tcb_corres:
+  "corres dc
+  (invs and valid_sched and simple_sched_action
+        and bound_sc_tcb_at ((=) None) t
+        and sc_tcb_sc_at ((=) None) ptr
+        and ex_nonz_cap_to t and ex_nonz_cap_to ptr)
+  (\<lambda>s. invs' s \<and> ex_nonz_cap_to' t s \<and> ex_nonz_cap_to' ptr s)
+  (sched_context_bind_tcb ptr t) (schedContextBindTCB ptr t)"
+  apply (simp only: sched_context_bind_tcb_def schedContextBindTCB_def)
+  apply (rule stronger_corres_guard_imp)
+    apply clarsimp
+    apply (rule corres_symb_exec_r')
+       apply (rule corres_split_nor)
+          apply (rule corres_split_nor)
+             apply (rule corres_split_nor)
+                apply (rule_tac r'="(=)" in corres_split)
+                   apply (rule corres_when, simp)
+                   apply (rule corres_split_nor)
+                      apply (rule rescheduleRequired_corres)
+                     apply (rule tcbSchedEnqueue_corres)
+                    apply wp
+                   apply wp
+                  apply (rule isSchedulable_corres)
+                 apply (wpsimp simp: is_schedulable_def)
+                apply (wpsimp wp: threadGet_wp getTCB_wp simp: isSchedulable_def inReleaseQueue_def)
+               apply (rule sched_context_resume_corres)
+              apply (rule_tac Q="\<lambda>rv s. invs s \<and> weak_valid_sched_action s \<and>
+                                        sc_tcb_sc_at ((=) (Some t)) ptr s \<and>
+                                        bound_sc_tcb_at (\<lambda>sc. sc = Some ptr) t s"
+                           in hoare_strengthen_post[rotated], fastforce)
+              apply (wp sched_context_resume_weak_valid_sched_action sched_context_resume_pred_tcb_at)
+             apply (rule_tac Q="\<lambda>_. invs'" in hoare_strengthen_post[rotated], fastforce)
+             apply (wp schedContextResume_invs')
+            apply (rule_tac f'="scTCB_update (\<lambda>_. Some t)"
+                         in update_sc_no_reply_stack_update_ko_at'_corres; clarsimp)
+             apply (clarsimp simp: sc_relation_def)
+            apply (clarsimp simp: objBits_def objBitsKO_def)
+           apply (simp add: pred_conj_def invs_def valid_state_def  cong: conj_cong)
+           apply (wpsimp wp: valid_irq_node_typ obj_set_prop_at get_sched_context_wp ssc_refs_of_Some
+                             update_sched_context_valid_objs_same valid_ioports_lift
+                             update_sched_context_iflive_update update_sched_context_refs_of_update
+                             update_sched_context_cur_sc_tcb_None update_sched_context_valid_idle
+                       simp: invs'_def valid_state'_def valid_pspace_def
+                  | rule hoare_vcg_conj_lift update_sched_context_wp)+
+         apply (clarsimp simp: set_tcb_obj_ref_thread_set sc_relation_def)
+         apply (rule threadset_corres; clarsimp simp: tcb_relation_def)
+        apply (clarsimp simp: pred_conj_def)
+        apply ((wp set_tcb_sched_context_valid_ready_qs_not_queued
+                   set_tcb_sched_context_valid_release_q_not_queued
+                   set_tcb_sched_context_simple_weak_valid_sched_action
+               | ((rule hoare_vcg_conj_lift)?, rule set_tcb_obj_ref_wp))+)[1]
+       apply (clarsimp simp: pred_conj_def valid_pspace'_def cong: conj_cong)
+       apply (wp threadSet_valid_objs' threadSet_valid_queues threadSet_valid_queues'
+                 threadSet_iflive' threadSet_not_inQ threadSet_ifunsafe'T threadSet_idle'T
+                 threadSet_sch_actT_P[where P=False, simplified] threadSet_ctes_ofT threadSet_mdb'
+                 threadSet_valid_release_queue threadSet_valid_release_queue' valid_irq_node_lift
+                 valid_irq_handlers_lift'' untyped_ranges_zero_lift threadSet_valid_dom_schedule'
+                 threadSet_ct_idle_or_in_cur_domain' threadSet_cur
+              | clarsimp simp: tcb_cte_cases_def cteCaps_of_def
+              | rule hoare_vcg_conj_lift threadSet_wp refl)+
+   apply (clarsimp simp: invs_def valid_state_def valid_pspace_def valid_sched_def)
+   apply (intro conjI impI allI; (solves clarsimp)?)
+              apply (fastforce simp: valid_obj_def obj_at_def sc_at_ppred_def is_sc_obj_def)
+             apply (clarsimp simp: valid_sched_context_def obj_at_def pred_tcb_at_def is_tcb_def)
+            apply (fastforce simp: obj_at_def pred_tcb_at_def sc_at_ppred_def tcb_cap_cases_def
+                             elim: ex_cap_to_after_update)
+           apply (fastforce simp: obj_at_def pred_tcb_at_def sc_at_ppred_def
+                                  tcb_st_refs_of_def state_refs_of_def
+                            elim: delta_sym_refs split: if_splits)
+          apply (fastforce dest: idle_no_ex_cap)
+         apply (fastforce dest: idle_sc_no_ex_cap)
+        apply (fastforce simp: tcb_at_kh_simps pred_map_eq_def
+                        elim!: valid_ready_qs_no_sc_not_queued)
+       apply (fastforce simp: tcb_at_kh_simps pred_map_eq_def
+                       elim!: valid_release_q_no_sc_not_in_release_q)
+      apply (fastforce simp: sc_at_pred_def sc_at_ppred_def obj_at_def bound_sc_tcb_at_def
+                      split: if_splits)
+     apply (clarsimp simp: weak_valid_sched_action_def simple_sched_action_def)
+    apply (clarsimp simp: sc_at_ppred_def obj_at_def bound_sc_tcb_at_def)
+   apply (clarsimp simp: sc_at_ppred_def obj_at_def bound_sc_tcb_at_def)
+  apply (subgoal_tac "obj_at' (\<lambda>sc. scTCB sc = None) ptr s'")
+   apply (subgoal_tac "bound_sc_tcb_at' ((=) None) t s'")
+    apply (subgoal_tac "ptr \<noteq> idle_sc_ptr")
+     apply (clarsimp simp: invs'_def valid_state'_def valid_pspace'_def pred_tcb_at'_def
+                           sc_at_ppred_def obj_at'_def projectKO_eq projectKO_tcb projectKO_sc)
+     apply (intro conjI allI impI; (solves \<open>clarsimp simp: inQ_def comp_def\<close>)?)
+              apply (clarsimp simp: valid_tcb'_def tcb_cte_cases_def obj_at'_def projectKO_eq)
+             apply (clarsimp simp: tcb_cte_cases_def)
+            apply (fastforce simp: valid_obj'_def valid_sched_context'_def tcb_cte_cases_def
+                                   obj_at'_def projectKO_eq projectKO_sc projectKO_tcb)
+           apply (fastforce elim: valid_objs_sizeE'[OF valid_objs'_valid_objs_size']
+                            simp: objBits_def objBitsKO_def valid_obj_size'_def
+                                  valid_sched_context_size'_def)
+          apply (fastforce elim: ex_cap_to'_after_update simp: ko_wp_at'_def tcb_cte_cases_def)
+         apply (clarsimp simp: idle_tcb'_2_def)
+        apply (clarsimp simp: valid_release_queue'_def obj_at'_def projectKO_eq projectKO_tcb)
+       apply (clarsimp simp: valid_release_queue'_def obj_at'_def projectKO_eq projectKO_tcb)
+      apply (clarsimp simp: untyped_ranges_zero_inv_def cteCaps_of_def comp_def)
+     apply simp
+    apply (fastforce simp: invs'_def valid_state'_def dest: global'_sc_no_ex_cap)
+   apply (clarsimp simp: state_relation_def invs_def valid_state_def valid_pspace_def)
+   apply (subgoal_tac "tcb_at' t s'")
+    apply (clarsimp simp: pspace_relation_def pred_tcb_at_def pred_tcb_at'_def obj_at_def obj_at'_def)
+    apply (drule_tac x=t in bspec; clarsimp simp: other_obj_relation_def tcb_relation_def projectKOs)
+   apply (fastforce elim: tcb_at_cross)
+  apply (clarsimp simp: sc_relation_def state_relation_def invs_def valid_state_def valid_pspace_def)
+  apply (subgoal_tac "sc_at' ptr s'")
+   apply (clarsimp simp: obj_at_def sc_at_pred_n_def obj_at'_def projectKOs pspace_relation_def)
+   apply (drule_tac x=ptr in bspec; clarsimp simp: sc_relation_def split: if_splits)
+  apply (fastforce simp: sc_at_pred_n_def obj_at_def is_sc_obj_def valid_obj_def elim!: sc_at_cross)
+  done
+
+schematic_goal finaliseSlot'_def:
+  "finaliseSlot' a b = ?X"
+  by (rule ext) simp
+
+lemma cteDelete_fh_lift:
+  assumes A: "\<And>x. \<lbrace>Q\<rbrace> emptySlot target x \<lbrace>\<lambda>_. P\<rbrace>"
+  and     B: "\<And>x. \<lbrace>R\<rbrace> cancelAllIPC x \<lbrace>\<lambda>_. Q\<rbrace>"
+  and     C: "\<And>s. (P and invs'  and L) s \<Longrightarrow> Q s \<and> R s"
+  shows "\<lbrace>P and invs' and cte_wp_at' (isValidFaultHandler \<circ> cteCap) target and L\<rbrace>
+         cteDelete target True
+         \<lbrace>\<lambda>_. P\<rbrace>"
+  apply (wpsimp wp: A simp: cteDelete_def)
+   prefer 2
+   apply assumption
+  apply (subst finaliseSlot_def)
+  apply (subst finaliseSlot'_def)
+  apply (rule hoare_vcg_seqE[rotated])
+   apply (subst liftE_validE)
+   apply (rule getCTE_sp)
+  apply (clarsimp split del: if_split)
+  apply (rule_tac Q="P and invs' and L and cte_wp_at' (\<lambda>c. c = cte) target
+                       and K (isValidFaultHandler (cteCap cte))" in hoare_pre(2))
+   apply (case_tac "cteCap cte"; clarsimp simp: isValidFaultHandler_def split: bool.splits)
+    apply (wpsimp simp: C)+
+         apply (rule hoare_FalseE)
+        apply (rule hoare_FalseE)
+       apply (rule hoare_FalseE)
+      apply (wpsimp wp: B isFinal simp: capRemovable_def finaliseCap_def isEndpointCap_def)+
+   apply (fastforce simp: C cte_wp_at'_def final_matters'_def
+                          capRemovable_def invs'_def valid_state'_def)+
+  done
+
+lemma hoare_vcg_common_conj_liftE:
+  "\<lbrakk>\<lbrace>Q\<rbrace> f \<lbrace>\<lambda>_. A\<rbrace>; \<lbrace>R\<rbrace> f \<lbrace>B\<rbrace>,\<lbrace>C\<rbrace>\<rbrakk> \<Longrightarrow> \<lbrace>Q and R\<rbrace> f \<lbrace>\<lambda>rv. A and B rv\<rbrace>,\<lbrace>\<lambda>rv. A and C rv\<rbrace>"
+  by (fastforce simp: valid_def validE_def split: sum.split)
+
+lemma installTCBCap_ex_nonz_cap_to':
+  "\<lbrace>\<lambda>s. ex_nonz_cap_to' p s \<and> invs' s \<and> \<not>ep_at' p s \<and>
+        cte_wp_at' (isValidFaultHandler \<circ> cteCap) (cte_map (target, tcb_cnode_index 3)) s\<rbrace>
+   installTCBCap target slot 3 slot_opt
+   \<lbrace>\<lambda>rv. ex_nonz_cap_to' p\<rbrace>"
+  unfolding installTCBCap_def getThreadFaultHandlerSlot_def locateSlotTCB_def locateSlotBasic_def
+  apply (case_tac slot_opt; clarsimp)
+   apply wpsimp
+  apply (rule validE_valid)
+  apply (rule hoare_vcg_seqE[rotated])
+   apply (rule liftE_wp[OF hoare_return_sp])
+  apply (rule valid_validE)
+  apply (rule hoare_gen_asm)
+  apply (clarsimp simp: objBits_def objBitsKO_def)
+  apply (wpsimp wp: checkCap_wp assertDerived_wp_weak cteInsert_cap_to')
+   apply (rule_tac Q="\<lambda>_. ex_nonz_cap_to' p and
+                          cte_wp_at' (\<lambda>c. cteCap c = capability.NullCap)
+                                       (target + 2 ^ cteSizeBits * tcbFaultHandlerSlot)"
+               and E="\<lambda>_. ex_nonz_cap_to' p and \<top>" in hoare_post_impErr)
+     apply (rule hoare_vcg_common_conj_liftE)
+      apply (rule cteDelete_fh_lift)
+        apply (wpsimp wp: hoare_vcg_ex_lift emptySlot_cte_wp_cap_other simp: ex_nonz_cap_to'_def)
+       apply (wpsimp wp: hoare_vcg_ex_lift)
+      apply (clarsimp simp: ex_nonz_cap_to'_def)
+      apply (rule_tac x=cref in exI)
+      apply clarsimp
+      apply (prop_tac "\<not> ep_at' p s \<and> cte_wp_at' (isValidFaultHandler \<circ> cteCap)
+                                                  (target + 2 ^ cteSizeBits * tcbFaultHandlerSlot) s")
+       apply assumption
+      apply (clarsimp simp: cte_wp_at_ctes_of)
+      apply (prop_tac "s \<turnstile>' (cteCap cte)")
+       apply fastforce
+      apply (prop_tac "\<not> isEndpointCap (cteCap cte)")
+       apply (fastforce simp: valid_cap'_def isCap_simps)
+      apply (case_tac "cteCap cte"; clarsimp simp: isValidFaultHandler_def isEndpointCap_def)
+     apply (rule hoare_validE_cases; rule hoare_pre)
+        apply (wpsimp wp: cteDelete_deletes)+
+  apply (clarsimp simp: comp_def cte_map_def tcb_cnode_index_def
+                        objBits_defs cte_level_bits_def tcbFaultHandlerSlot_def)
+  done
+
+lemma threadSetPriority_ex_nonz_cap_to'[wp]:
+  "threadSetPriority param_a param_b \<lbrace>ex_nonz_cap_to' p\<rbrace>"
+  by (wpsimp wp: threadSet_cap_to' simp: threadSetPriority_def)
+
+crunches setPriority
+  for ex_nonz_cap_to'[wp]: "ex_nonz_cap_to' p"
+  (wp: crunch_wps simp: crunch_simps)
+
+crunches setMCPriority
+  for tcb_at'[wp]: "tcb_at' t"
+  and weak_sch_act_wf[wp]: "\<lambda>s. weak_sch_act_wf (ksSchedulerAction s) s"
+  (wp: crunch_wps simp: crunch_simps inQ_def)
+
+lemma setMCPriority_ex_nonz_cap_to'[wp]:
+  "setMCPriority param_a param_b \<lbrace>ex_nonz_cap_to' p\<rbrace>"
+  by (wpsimp wp: threadSet_cap_to' simp: setMCPriority_def)
+
+lemma mapTCBPtr_threadGet: "mapTCBPtr t f = threadGet f t"
+  by (clarsimp simp: mapTCBPtr_def threadGet_def liftM_def)
+
+lemma monadic_rewrite_bind_unbind:
+  "monadic_rewrite False True (tcb_at t)
+   (case sc_opt of None \<Rightarrow> return ()
+                 | Some None \<Rightarrow> maybe_sched_context_unbind_tcb t
+                 | Some (Some sc_ptr) \<Rightarrow> maybe_sched_context_bind_tcb sc_ptr t)
+   (do y <- get_tcb_obj_ref tcb_sched_context t;
+       case sc_opt of None \<Rightarrow> return ()
+                    | Some None \<Rightarrow> case y of None \<Rightarrow> return ()
+                                           | Some x \<Rightarrow> sched_context_unbind_tcb x
+                    | Some (Some sc_ptr) \<Rightarrow> when (y \<noteq> Some sc_ptr) $ sched_context_bind_tcb sc_ptr t
+    od)"
+  apply (case_tac sc_opt; clarsimp)
+   apply (clarsimp simp: monadic_rewrite_def bind_def get_tcb_obj_ref_def thread_get_def
+                         gets_the_def get_tcb_def gets_def get_def obj_at_def is_tcb_def)
+   apply (case_tac ko; clarsimp simp: return_def)
+  apply (case_tac a; clarsimp simp: maybeM_def maybe_sched_context_unbind_tcb_def
+                                    maybe_sched_context_bind_tcb_def monadic_rewrite_def)
+  done
 
 lemma tc_corres_sched:
   fixes t slot sc_fault_h p_auth mcp_auth sc_opt sl' sc_fault_h' sc_opt'
-  defines "tc_inv_sched \<equiv> tcb_invocation.ThreadControlSched t slot sc_fault_h p_auth mcp_auth sc_opt"
+  defines "tc_inv_sched \<equiv> tcb_invocation.ThreadControlSched t slot sc_fault_h mcp_auth p_auth sc_opt"
   defines "tc_inv_sched' \<equiv> ThreadControlSched t sl' sc_fault_h' p_auth mcp_auth sc_opt'"
   assumes "tcbinv_relation tc_inv_sched tc_inv_sched'"
   shows
-    "corres (intr \<oplus> (=))
-    (einvs and simple_sched_action and tcb_at t and
-     (\<lambda>s. sc_fault_h \<noteq> None \<longrightarrow> cte_at slot s) and
-     case_option \<top> (valid_cap o fst) sc_fault_h and
-     case_option \<top> (cte_at o snd) sc_fault_h and
-     case_option \<top> (no_cap_to_obj_dr_emp o fst) sc_fault_h and
-     (\<lambda>s. case_option True (\<lambda>(pr, auth). mcpriority_tcb_at (\<lambda>m. pr \<le> m) auth s) p_auth) and \<comment> \<open>only set prio \<le> mcp\<close>
-     (\<lambda>s. case_option True (\<lambda>(mcp, auth). mcpriority_tcb_at (\<lambda>m. mcp \<le> m) auth s) mcp_auth) \<comment> \<open>only set mcp \<le> prev_mcp\<close>)
+    "corres (dc \<oplus> (=))
+    (einvs and simple_sched_action and cte_at slot and tcb_inv_wf tc_inv_sched
+           and (\<lambda>s. p_auth \<noteq> None \<longrightarrow> ct_released s \<and> ct_active s \<and> ct_not_in_release_q s))
     (invs' and sch_act_simple and tcb_inv_wf' tc_inv_sched')
     (invoke_tcb tc_inv_sched)
     (invokeTCB tc_inv_sched')"
-  sorry (* FIXME RT: use Tcb_AI.tcb_inv_wf on abstract side *)
-(* FIXME RT: old tc_corres proof, now only covers sched case
-proof -
-  have P: "\<And>t v. corres dc
-               (tcb_at t)
-               (tcb_at' t)
-               (option_update_thread t (tcb_fault_handler_update o (%x _. x))
-               (option_map to_bl v))
-               (case v of None \<Rightarrow> return ()
-                 | Some x \<Rightarrow> threadSet (tcbFaultHandler_update (%_. x)) t)"
-    apply (rule out_corres, simp_all add: exst_same_def)
-    apply (case_tac v, simp_all add: out_rel_def)
-    apply (safe, case_tac tcb', simp add: tcb_relation_def split: option.split)
-    done
-  have R: "\<And>t v. corres dc
-               (tcb_at t)
-               (tcb_at' t)
-               (option_update_thread t (tcb_ipc_buffer_update o (%x _. x)) v)
-               (case v of None \<Rightarrow> return ()
-                 | Some x \<Rightarrow> threadSet (tcbIPCBuffer_update (%_. x)) t)"
-    apply (rule out_corres, simp_all add: exst_same_def)
-    apply (case_tac v, simp_all add: out_rel_def)
-    apply (safe, case_tac tcb', simp add: tcb_relation_def)
-    done
-  have S: "\<And>t x. corres dc (einvs and tcb_at t) (invs' and tcb_at' t and valid_objs' and K (valid_option_prio p_auth))
-                   (case_option (return ()) (\<lambda>(p, auth). set_priority t p) p_auth)
-                   (case_option (return ()) (\<lambda>p'. setPriority t (fst p')) p_auth)"
-    apply (case_tac p_auth; clarsimp simp: sp_corres)
-    done
-  have S': "\<And>t x. corres dc (tcb_at t) (tcb_at' t)
-                    (case_option (return ()) (\<lambda>(mcp, auth). set_mcpriority t mcp) mcp_auth)
-                    (case_option (return ()) (\<lambda>mcp'. setMCPriority t (fst mcp')) mcp_auth)"
-    apply(case_tac mcp_auth; clarsimp simp: smcp_corres)
-    done
-  have T: "\<And>x x' ref getfn target.
-      \<lbrakk> newroot_rel x x'; getfn = return (cte_map (target, ref));
-             x \<noteq> None \<longrightarrow> {e, f, option_map undefined g} \<noteq> {None} \<rbrakk> \<Longrightarrow>
-      corres (intr \<oplus> dc)
-
-             (einvs and simple_sched_action and cte_at (target, ref) and emptyable (target, ref) and
-              (\<lambda>s. \<forall>(sl, c) \<in> (case x of None \<Rightarrow> {} | Some (c, sl) \<Rightarrow> {(sl, c), (slot, c)}).
-                        cte_at sl s \<and> no_cap_to_obj_dr_emp c s \<and> valid_cap c s)
-              and K (case x of None \<Rightarrow> True
-                       | Some (c, sl) \<Rightarrow> is_cnode_or_valid_arch c))
-             (invs' and sch_act_simple and cte_at' (cte_map (target, ref)) and
-              (\<lambda>s. \<forall>cp \<in> (case x' of None \<Rightarrow> {} | Some (c, sl) \<Rightarrow> {c}). s \<turnstile>' cp))
-          (case x of None \<Rightarrow> returnOk ()
-           | Some pr \<Rightarrow> case_prod (\<lambda>new_cap src_slot.
-               doE cap_delete (target, ref);
-                   liftE $ check_cap_at new_cap src_slot $
-                           check_cap_at (cap.ThreadCap target) slot $
-                           cap_insert new_cap src_slot (target, ref)
-               odE) pr)
-          (case x' of
-              None \<Rightarrow> returnOk ()
-              | Some pr \<Rightarrow> (\<lambda>(newCap, srcSlot).
-                  do slot \<leftarrow> getfn;
-                     doE uu \<leftarrow> cteDelete slot True;
-                         liftE (checkCapAt newCap srcSlot
-                               (checkCapAt (capability.ThreadCap target) sl'
-                               (assertDerived srcSlot newCap (cteInsert newCap srcSlot slot))))
-                     odE
-                  od) pr)"
-    apply (case_tac "x = None")
-     apply (simp add: newroot_rel_def returnOk_def)
-    apply (drule(1) mp, drule mp [OF sl])
-    apply (clarsimp simp add: newroot_rel_def returnOk_def split_def)
-    apply (rule corres_gen_asm)
-    apply (rule corres_guard_imp)
-      apply (rule corres_split_norE [OF _ cap_delete_corres])
-        apply (simp del: dc_simp)
-        apply (erule checked_insert_corres)
-       apply (fold validE_R_def)
-       apply (wp cap_delete_deletes cap_delete_cte_at cap_delete_valid_cap
-                    | strengthen use_no_cap_to_obj_asid_strg)+
-      apply (wp cteDelete_invs' cteDelete_deletes)
-     apply (clarsimp dest!: is_cnode_or_valid_arch_cap_asid)
-    apply clarsimp
-    done
-  have U2: "getThreadBufferSlot a = return (cte_map (a, tcb_cnode_index 4))"
-    by (simp add: getThreadBufferSlot_def locateSlot_conv
-                  cte_map_def tcb_cnode_index_def tcbIPCBufferSlot_def
-                  cte_level_bits_def)
-  have T2: "corres (intr \<oplus> dc)
-     (einvs and simple_sched_action and tcb_at a and
-         (\<lambda>s. \<forall>(sl, c) \<in> (case g of None \<Rightarrow> {} | Some (x, v) \<Rightarrow> {(slot, cap.NullCap)} \<union>
-             (case v of None \<Rightarrow> {} | Some (c, sl) \<Rightarrow> {(sl, c), (slot, c)})).
-                   cte_at sl s \<and> no_cap_to_obj_dr_emp c s \<and> valid_cap c s)
-         and K (case g of None \<Rightarrow> True | Some (x, v) \<Rightarrow> (case v of
-                   None \<Rightarrow> True | Some (c, sl) \<Rightarrow> is_cnode_or_valid_arch c
-                                                 \<and> is_arch_cap c
-                                                 \<and> valid_ipc_buffer_cap c x
-                                                 \<and> is_aligned x msg_align_bits)))
-     (invs' and sch_act_simple and tcb_at' a and
-       (\<lambda>s. \<forall>cp \<in> (case g' of None \<Rightarrow> {} | Some (x, v) \<Rightarrow> (case v of
-                              None \<Rightarrow> {} | Some (c, sl) \<Rightarrow> {c})). s \<turnstile>' cp) and
-       K (case g' of None \<Rightarrow> True | Some (x, v) \<Rightarrow> is_aligned x msg_align_bits
-       \<and> (case v of None \<Rightarrow> True | Some (ac, _) \<Rightarrow> isArchObjectCap ac)) )
-     (case_option (returnOk ())
-       (case_prod
-         (\<lambda>ptr frame.
-             doE cap_delete (a, tcb_cnode_index 4);
-                 do y \<leftarrow> thread_set (tcb_ipc_buffer_update (\<lambda>_. ptr)) a;
-                    y \<leftarrow> case_option (return ())
-                          (case_prod
-                          (\<lambda>new_cap src_slot.
-                            check_cap_at new_cap src_slot $
-                            check_cap_at (cap.ThreadCap a) slot $
-                            cap_insert new_cap src_slot (a, tcb_cnode_index 4)))
-                          frame;
-                    cur \<leftarrow> gets cur_thread;
-                    liftE $ when (cur = a) (reschedule_required)
-                 od
-             odE))
-       g)
-     (case_option (returnOk ())
-        (\<lambda>(ptr, frame).
-            do bufferSlot \<leftarrow> getThreadBufferSlot a;
-            doE y \<leftarrow> cteDelete bufferSlot True;
-            do y \<leftarrow> threadSet (tcbIPCBuffer_update (\<lambda>_. ptr)) a;
-               y \<leftarrow> (case_option (return ())
-                      (case_prod
-                        (\<lambda>newCap srcSlot.
-                            checkCapAt newCap srcSlot $
-                            checkCapAt
-                             (capability.ThreadCap a)
-                             sl' $
-                            assertDerived srcSlot newCap $
-                            cteInsert newCap srcSlot bufferSlot))
-                      frame);
-               cur \<leftarrow> getCurThread;
-               liftE $ when (cur = a) rescheduleRequired
-            od odE od)
-        g')" (is "corres _ ?T2_pre ?T2_pre' _ _")
-    using z sl
-    apply -
-    apply (rule corres_guard_imp[where P=P and P'=P'
-                                  and Q="P and cte_at (a, tcb_cnode_index 4)"
-                                  and Q'="P' and cte_at' (cte_map (a, cap))" for P P' a cap])
-      apply (cases g)
-       apply (simp, simp add: returnOk_def)
-      apply (clarsimp simp: liftME_def[symmetric] U2 liftE_bindE)
-      apply (case_tac b, simp_all add: newroot_rel_def)
-       apply (rule corres_guard_imp)
-         apply (rule corres_split_norE)
-            apply (rule_tac F="is_aligned aa msg_align_bits" in corres_gen_asm2)
-            apply (rule corres_split_nor)
-               apply (rule corres_split [OF _ gct_corres], clarsimp)
-                 apply (rule corres_when[OF refl rescheduleRequired_corres])
-                apply (wpsimp wp: gct_wp)+
-              apply (rule threadset_corres,
-                      (simp add: tcb_relation_def), (simp add: exst_same_def)+)[1]
-             apply (wp hoare_drop_imp)
-             apply (rule threadcontrol_corres_helper1[unfolded pred_conj_def])
-            apply simp
-            apply (wp hoare_drop_imp)
-            apply (wp threadcontrol_corres_helper2 | wpc | simp)+
-           apply (rule cap_delete_corres)
-          apply wp
-         apply (wpsimp wp: cteDelete_invs' hoare_vcg_conj_lift)
-        apply (fastforce simp: emptyable_def)
-       apply fastforce
-      apply clarsimp
-      apply (rule corres_guard_imp)
-        apply (rule corres_split_norE [OF _ cap_delete_corres])
-          apply (rule_tac F="is_aligned aa msg_align_bits" in corres_gen_asm)
-          apply (rule_tac F="isArchObjectCap ac" in corres_gen_asm2)
+  using assms
+  apply -
+  apply (simp add: invokeTCB_def liftE_bindE bind_assoc maybeM_def)
+  apply (rule stronger_corres_guard_imp)
+    apply (rule corres_split_norE)
+       apply (rule corres_split_nor)
           apply (rule corres_split_nor)
+             apply (simp add: bind_assoc[symmetric])
              apply (rule corres_split_nor)
-                apply (rule corres_split [OF _ gct_corres], clarsimp)
-                  apply (rule corres_when[OF refl rescheduleRequired_corres])
-                 apply (wp gct_wp)+
-               apply (erule checked_insert_corres)
-              apply (wp hoare_drop_imp threadcontrol_corres_helper3)[1]
-             apply (wp hoare_drop_imp threadcontrol_corres_helper4)[1]
-            apply (rule threadset_corres,
-                   simp add: tcb_relation_def, (simp add: exst_same_def)+)
-           apply (wp thread_set_tcb_ipc_buffer_cap_cleared_invs
-                     thread_set_cte_wp_at_trivial thread_set_not_state_valid_sched
-                  | simp add: ran_tcb_cap_cases)+
-          apply (wp threadSet_invs_trivial
-                    threadSet_cte_wp_at' | simp)+
-         apply (wp cap_delete_deletes cap_delete_cte_at
-                   cap_delete_valid_cap cteDelete_deletes
-                   cteDelete_invs'
-                | strengthen use_no_cap_to_obj_asid_strg
-                | clarsimp simp: inQ_def inQ_tc_corres_helper)+
-       apply (clarsimp simp: cte_wp_at_caps_of_state
-                      dest!: is_cnode_or_valid_arch_cap_asid)
-       apply (clarsimp simp: emptyable_def)
-      apply (clarsimp simp: inQ_def)
-     apply (clarsimp simp: obj_at_def is_tcb)
-     apply (rule cte_wp_at_tcbI, simp, fastforce, simp)
-    apply (clarsimp simp: cte_map_def tcb_cnode_index_def obj_at'_def
-                          projectKOs objBits_simps)
-    apply (erule(2) cte_wp_at_tcbI', fastforce simp: objBits_defs cte_level_bits_def, simp)
-    done
-  have U: "getThreadCSpaceRoot a = return (cte_map (a, tcb_cnode_index 0))"
-    apply (clarsimp simp add: getThreadCSpaceRoot)
-    apply (simp add: cte_map_def tcb_cnode_index_def
-                     cte_level_bits_def word_bits_def)
-    done
-  have V: "getThreadVSpaceRoot a = return (cte_map (a, tcb_cnode_index 1))"
-    apply (clarsimp simp add: getThreadVSpaceRoot)
-    apply (simp add: cte_map_def tcb_cnode_index_def to_bl_1 objBits_defs
-                     cte_level_bits_def word_bits_def)
-    done
-  have X: "\<And>x P Q R M. (\<And>y. x = Some y \<Longrightarrow> \<lbrace>P y\<rbrace> M y \<lbrace>Q\<rbrace>,\<lbrace>R\<rbrace>)
-               \<Longrightarrow> \<lbrace>case_option (Q ()) P x\<rbrace> case_option (returnOk ()) M x \<lbrace>Q\<rbrace>,\<lbrace>R\<rbrace>"
-    by (case_tac x, simp_all, wp)
-  have Y: "\<And>x P Q M. (\<And>y. x = Some y \<Longrightarrow> \<lbrace>P y\<rbrace> M y \<lbrace>Q\<rbrace>,-)
-               \<Longrightarrow> \<lbrace>case_option (Q ()) P x\<rbrace> case_option (returnOk ()) M x \<lbrace>Q\<rbrace>,-"
-    by (case_tac x, simp_all, wp)
-  have Z: "\<And>P f R Q x. \<lbrace>P\<rbrace> f \<lbrace>\<lambda>rv. Q and R\<rbrace> \<Longrightarrow> \<lbrace>P\<rbrace> f \<lbrace>\<lambda>rv. case_option Q (\<lambda>y. R) x\<rbrace>"
-    apply (rule hoare_post_imp)
-     defer
-     apply assumption
-    apply (case_tac x, simp_all)
-    done
-  have A: "\<And>x P Q M. (\<And>y. x = Some y \<Longrightarrow> \<lbrace>P y\<rbrace> M y \<lbrace>Q\<rbrace>)
-               \<Longrightarrow> \<lbrace>case_option (Q ()) P x\<rbrace> case_option (return ()) M x \<lbrace>Q\<rbrace>"
-    by (case_tac x, simp_all, wp)
-  have B: "\<And>t v. \<lbrace>invs' and tcb_at' t\<rbrace> threadSet (tcbFaultHandler_update v) t \<lbrace>\<lambda>rv. invs'\<rbrace>"
-    by (wp threadSet_invs_trivial | clarsimp simp: inQ_def)+
-  note stuff = Z B out_invs_trivial hoare_case_option_wp
-    hoare_vcg_const_Ball_lift hoare_vcg_const_Ball_lift_R
-    cap_delete_deletes cap_delete_valid_cap out_valid_objs
-    cap_insert_objs
-    cteDelete_deletes cteDelete_sch_act_simple
-    out_valid_cap out_cte_at out_tcb_valid out_emptyable
-    CSpaceInv_AI.cap_insert_valid_cap cap_insert_cte_at cap_delete_cte_at
-    cap_delete_tcb cteDelete_invs' checkCap_inv [where P="valid_cap' c0" for c0]
-    check_cap_inv[where P="tcb_at p0" for p0] checkCap_inv [where P="tcb_at' p0" for p0]
-    check_cap_inv[where P="cte_at p0" for p0] checkCap_inv [where P="cte_at' p0" for p0]
-    check_cap_inv[where P="valid_cap c" for c] checkCap_inv [where P="valid_cap' c" for c]
-    check_cap_inv[where P="tcb_cap_valid c p1" for c p1]
-    check_cap_inv[where P=valid_sched]
-    check_cap_inv[where P=simple_sched_action]
-    checkCap_inv [where P=sch_act_simple]
-    out_no_cap_to_trivial [OF ball_tcb_cap_casesI]
-    checked_insert_no_cap_to
-  note if_cong [cong] option.case_cong [cong]
-  show ?thesis
-    apply (simp add: invokeTCB_def liftE_bindE)
-    apply (simp only: eq_commute[where a= "a"])
-    apply (rule corres_guard_imp)
-      apply (rule corres_split_nor [OF _ P])
-        apply (rule corres_split_nor[OF _ S', simplified])
-          apply (rule corres_split_norE [OF _ T [OF x U], simplified])
-            apply (rule corres_split_norE [OF _ T [OF y V], simplified])
-              apply (rule corres_split_norE)
-                 apply (rule corres_split_nor [OF _ S, simplified])
-                   apply (rule corres_returnOkTT, simp)
-                  apply wp
-                 apply wp
-                apply (rule T2[simplified])
-               apply (wpsimp wp: hoare_vcg_const_imp_lift_R hoare_vcg_const_imp_lift
-                                 hoare_vcg_all_lift_R hoare_vcg_all_lift as_user_invs cap_delete_deletes
-                                 thread_set_ipc_tcb_cap_valid thread_set_tcb_ipc_buffer_cap_cleared_invs
-                                 thread_set_cte_wp_at_trivial thread_set_valid_cap cap_delete_valid_cap
-                                 reschedule_preserves_valid_sched thread_set_not_state_valid_sched
-                                 check_cap_inv[where P=valid_sched] (* from stuff *)
-                                 check_cap_inv[where P="tcb_at p0" for p0]
-                           simp: ran_tcb_cap_cases)
-                apply (strengthen use_no_cap_to_obj_asid_strg)
-                apply (wpsimp wp: cap_delete_cte_at cap_delete_valid_cap)
-               apply (wpsimp wp: hoare_drop_imps)
-              apply ((wpsimp wp: hoare_vcg_const_imp_lift hoare_vcg_imp_lift' hoare_vcg_all_lift
-                                       threadSet_cte_wp_at' threadSet_invs_trivialT2 cteDelete_invs'
-                                 simp: tcb_cte_cases_def), (fastforce+)[6])
-                  apply wpsimp
-                  apply (wpsimp wp: hoare_vcg_const_imp_lift hoare_drop_imps hoare_vcg_all_lift
-                                    threadSet_invs_trivialT2 threadSet_cte_wp_at'
-                              simp: tcb_cte_cases_def, (fastforce+)[6])
-                  apply wpsimp
-                  apply (wpsimp wp: hoare_vcg_const_imp_lift hoare_drop_imps hoare_vcg_all_lift
-                                    rescheduleRequired_invs' threadSet_cte_wp_at'
-                              simp: tcb_cte_cases_def)
-                 apply (wpsimp wp: hoare_vcg_const_imp_lift hoare_drop_imps hoare_vcg_all_lift
-                                   rescheduleRequired_invs' threadSet_invs_trivialT2 threadSet_cte_wp_at'
-                             simp: tcb_cte_cases_def, (fastforce+)[6])
-                 apply wpsimp
-                 apply (wpsimp wp: hoare_vcg_const_imp_lift hoare_drop_imps hoare_vcg_all_lift
-                                   rescheduleRequired_invs' threadSet_invs_trivialT2 threadSet_cte_wp_at'
-                             simp: tcb_cte_cases_def, (fastforce+)[6])
-                 apply wpsimp
-                 apply (wpsimp wp: hoare_vcg_const_imp_lift hoare_drop_imps hoare_vcg_all_lift
-                                   rescheduleRequired_invs' threadSet_cap_to' threadSet_invs_trivialT2
-                                   threadSet_cte_wp_at' hoare_drop_imps
-                               simp: tcb_cte_cases_def)
-                apply (clarsimp)
-                apply ((wpsimp wp: stuff hoare_vcg_all_lift_R hoare_vcg_all_lift
-                                   hoare_vcg_const_imp_lift_R hoare_vcg_const_imp_lift
-                                   threadSet_valid_objs' thread_set_not_state_valid_sched
-                                   thread_set_tcb_ipc_buffer_cap_cleared_invs thread_set_cte_wp_at_trivial
-                                   thread_set_no_cap_to_trivial getThreadBufferSlot_dom_tcb_cte_cases
-                                   assertDerived_wp_weak threadSet_cap_to' out_pred_tcb_at_preserved
-                                   checkCap_wp assertDerived_wp_weak cap_insert_objs'
-                        | simp add: ran_tcb_cap_cases split_def U V
-                                  emptyable_def
-                        | strengthen tcb_cap_always_valid_strg
-                                   tcb_at_invs
-                                   use_no_cap_to_obj_asid_strg
-                        | (erule exE, clarsimp simp: word_bits_def))+)
-                apply (strengthen valid_tcb_ipc_buffer_update)
-                apply (strengthen invs_valid_objs')+
-                apply (wpsimp wp: cteDelete_invs' hoare_vcg_imp_lift' hoare_vcg_all_lift)
-               apply wpsimp
-              apply wpsimp
-             apply (clarsimp cong: imp_cong conj_cong simp: emptyable_def)
-             apply (rule_tac Q'="\<lambda>_. ?T2_pre" in hoare_post_imp_R[simplified validE_R_def, rotated])
-              (* beginning to deal with is_nondevice_page_cap *)
-              apply (clarsimp simp: emptyable_def is_nondevice_page_cap_simps is_cap_simps
-                                    is_cnode_or_valid_arch_def obj_ref_none_no_asid cap_asid_def
-                              cong: conj_cong imp_cong
-                             split: option.split_asm)
-              (* newly added proof scripts for dealing with is_nondevice_page_cap *)
-              apply (simp add: case_bool_If valid_ipc_buffer_cap_def is_nondevice_page_cap_arch_def
-                        split: arch_cap.splits if_splits)
-             (* is_nondevice_page_cap discharged *)
-             apply ((wp stuff checkCap_wp assertDerived_wp_weak cap_insert_objs'
-                     | simp add: ran_tcb_cap_cases split_def U V emptyable_def
-                     | wpc | strengthen tcb_cap_always_valid_strg use_no_cap_to_obj_asid_strg)+)[1]
-            apply (clarsimp cong: imp_cong conj_cong)
-            apply (rule_tac Q'="\<lambda>_. ?T2_pre' and (\<lambda>s. valid_option_prio p_auth)"
-                         in hoare_post_imp_R[simplified validE_R_def, rotated])
-             apply (case_tac g'; clarsimp simp: isCap_simps ; clarsimp elim: invs_valid_objs' cong:imp_cong)
-            apply (wp add: stuff hoare_vcg_all_lift_R hoare_vcg_all_lift
-                                 hoare_vcg_const_imp_lift_R hoare_vcg_const_imp_lift setMCPriority_invs'
-                                 threadSet_valid_objs' thread_set_not_state_valid_sched setP_invs'
-                                 threadSet_cap_to' out_pred_tcb_at_preserved assertDerived_wp
-                      del: cteInsert_invs
-                   | simp add: ran_tcb_cap_cases split_def U V
-                               emptyable_def
-                   | wpc | strengthen tcb_cap_always_valid_strg
-                                      use_no_cap_to_obj_asid_strg
-                   | wp (once) add: sch_act_simple_lift hoare_drop_imps del: cteInsert_invs
-                   | (erule exE, clarsimp simp: word_bits_def))+
-     (* the last two subgoals *)
-     apply (clarsimp simp: tcb_at_cte_at_0 tcb_at_cte_at_1[simplified] tcb_at_st_tcb_at[symmetric]
-                           tcb_cap_valid_def is_cnode_or_valid_arch_def invs_valid_objs emptyable_def
-                           obj_ref_none_no_asid no_cap_to_obj_with_diff_ref_Null is_valid_vtable_root_def
-                           is_cap_simps cap_asid_def vs_cap_ref_def arch_cap_fun_lift_def
-                     cong: conj_cong imp_cong
-                    split: option.split_asm)
-    by (clarsimp simp: invs'_def valid_state'_def valid_pspace'_def objBits_defs
-                       cte_map_tcb_0 cte_map_tcb_1[simplified] tcb_at_cte_at' cte_at_tcb_at_16'
-                       isCap_simps domIff valid_tcb'_def tcb_cte_cases_def arch_cap_fun_lift_def
-                split: option.split_asm
-                dest!: isValidVTableRootD)
-qed *)
+                apply (clarsimp simp: returnOk_def)
+               apply (rule monadic_rewrite_corres[OF _ monadic_rewrite_bind_unbind])
+               apply (rule_tac r'="(=)" in corres_split)
+                  apply (rule_tac P=\<top> and P'=\<top> in corres_option_split; clarsimp)
+                  apply (rule corres_option_split; clarsimp?)
+                   apply (rule_tac P=\<top> and P'=\<top> in corres_option_split; clarsimp)
+                   apply (rule sched_context_unbind_tcb_corres)
+                  apply (rule corres_when[OF _ sched_context_bind_tcb_corres], fastforce)
+                 apply (simp only: mapTCBPtr_threadGet get_tcb_obj_ref_def)
+                 apply (rule threadget_corres, clarsimp simp: tcb_relation_def)
+                apply (wp get_tcb_obj_ref_wp)
+               apply (wpsimp wp: getTCB_wp simp: mapTCBPtr_def)
+              apply (rule_tac P=\<top> in hoare_post_taut)
+             apply (rule hoare_post_taut)
+            apply (rule_tac P=\<top> and P'=\<top> in corres_option_split; clarsimp)
+            apply wpfix
+            apply (rule sp_corres2)
+           apply (rule_tac Q="\<lambda>_ s. invs s \<and> valid_sched s \<and> simple_sched_action s \<and>
+                                    tcb_at t s \<and> ex_nonz_cap_to t s \<and>
+                                    (\<forall>scPtr. sc_opt = Some (Some scPtr) \<longrightarrow>
+                                               ex_nonz_cap_to scPtr s \<and>
+                                               sc_tcb_sc_at ((=) None) scPtr s \<and>
+                                               bound_sc_tcb_at ((=) None) t s)"
+                        in hoare_strengthen_post[rotated])
+            apply (clarsimp simp: obj_at_def split: option.splits)
+            apply (frule invs_valid_objs)
+            apply (erule (1) valid_objsE)
+            apply (clarsimp simp: valid_obj_def valid_tcb_def obj_at_def is_sc_obj_def
+                                  invs_def valid_state_def valid_pspace_def)
+            apply (clarsimp split: Structures_A.kernel_object.splits)
+            apply (drule (2) bound_sc_tcb_bound_sc_at[where tcbptr=t])
+             apply (clarsimp simp: pred_tcb_at_def obj_at_def)
+            apply (clarsimp simp: sc_at_ppred_def obj_at_def)
+           apply (wpsimp wp: set_priority_valid_sched hoare_vcg_all_lift hoare_vcg_const_imp_lift)
+          apply (rule_tac Q=" \<lambda>_ s. invs' s \<and> tcb_at' t s \<and> ex_nonz_cap_to' t s \<and>
+                                   (\<forall>scPtr. sc_opt = Some (Some scPtr) \<longrightarrow> ex_nonz_cap_to' scPtr s)"
+                       in hoare_strengthen_post[rotated], fastforce split: option.split)
+          apply (wpsimp wp: setP_invs' hoare_vcg_all_lift hoare_vcg_const_imp_lift)
+         apply (rule_tac P=\<top> and P'=\<top> in corres_option_split; clarsimp)
+         apply (rule smcp_corres)
+        apply (rule_tac R="\<lambda>_. invs" in hoare_post_add)
+        apply (clarsimp simp: invs_cur case_option_If2 if_fun_split
+                        cong: conj_cong imp_cong split del: if_split)
+        apply (wpsimp wp: hoare_vcg_all_lift hoare_vcg_const_imp_lift)
+       apply (rule_tac R="\<lambda>_. invs'" in hoare_post_add)
+       apply (clarsimp simp: invs_queues invs_queues' invs_cur' case_option_If2 if_fun_split
+                       cong: conj_cong imp_cong split del: if_split)
+       apply (wpsimp wp: setMCPriority_invs' hoare_vcg_all_lift hoare_vcg_const_imp_lift)
+      apply (rule install_tcb_cap_corres; clarsimp)
+     apply (rule_tac Q="\<lambda>_ s. invs s \<and> valid_sched s \<and> simple_sched_action s \<and>
+                              tcb_at t s \<and> ex_nonz_cap_to t s \<and>
+                              (\<forall>scPtr. sc_opt = Some (Some scPtr) \<longrightarrow> ex_nonz_cap_to scPtr s \<and>
+                                                                      sc_tcb_sc_at ((=) None) scPtr s \<and>
+                                                                      bound_sc_tcb_at ((=) None) t s) \<and>
+                              (p_auth \<noteq> None \<longrightarrow> ct_released s \<and> ct_active s \<and> ct_not_in_release_q s)"
+                 and E="\<lambda>_. \<top>" in hoare_post_impErr[rotated], fastforce split: option.splits, simp)
+     apply (wp install_tcb_cap_invs install_tcb_cap_ex_nonz_cap_to hoare_vcg_all_lift hoare_vcg_const_imp_lift)
+     apply (rule valid_validE)
+     apply (rule hoare_lift_Pf2[where f="cur_thread"])
+      apply (wp install_tcb_cap_ct_active)
+     apply wp
+    apply (rule_tac Q=" \<lambda>_ s. invs' s \<and> tcb_at' t s \<and> ex_nonz_cap_to' t s \<and>
+                              (\<forall>scPtr. sc_opt = Some (Some scPtr) \<longrightarrow> ex_nonz_cap_to' scPtr s) \<and>
+                              (\<forall>p. p_auth = Some p \<longrightarrow> fst p \<le> maxPriority) \<and>
+                              (\<forall>p. mcp_auth = Some p \<longrightarrow> fst p \<le> maxPriority)"
+                and E="\<lambda>_. \<top>" in hoare_post_impErr[rotated], fastforce split: option.splits, simp)
+    apply (wp installTCBCap_invs' installTCBCap_ex_nonz_cap_to' hoare_vcg_all_lift hoare_vcg_const_imp_lift)
+   apply (subgoal_tac "(not ep_at t) s")
+    apply clarsimp
+    apply (fastforce simp: tcb_cap_valid_def pred_tcb_at_def pred_neg_def
+                           sc_at_ppred_def obj_at_def is_ep_def
+                     elim: cte_wp_at_weakenE dest: tcb_ep_slot_cte_wp_ats)
+   apply (clarsimp simp: pred_neg_def obj_at_def is_tcb_def is_ep_def)
+   apply (fastforce split: Structures_A.kernel_object.splits)
+  apply clarsimp
+  apply (subgoal_tac "cte_wp_at' (isValidFaultHandler \<circ> cteCap) (cte_map (t, tcb_cnode_index 3)) s'")
+   apply clarsimp
+   apply (intro conjI impI allI; clarsimp?)
+       apply (fastforce simp: tcb_at_cte_at'_3)
+      apply (clarsimp simp: newroot_rel_def)
+      apply (case_tac a; clarsimp simp: isCap_simps isValidFaultHandler_def
+                                        valid_fault_handler_def has_handler_rights_def)
+     apply (clarsimp simp: newroot_rel_def)
+     apply (case_tac a; clarsimp simp: isCap_simps isValidFaultHandler_def
+                                       valid_fault_handler_def has_handler_rights_def)
+    apply (clarsimp simp: obj_at'_def projectKO_eq projectKO_tcb projectKO_ep)
+   apply (clarsimp simp: obj_at'_def projectKO_eq projectKO_sc projectKO_ep)
+  apply (drule (1) tcb_ep_slot_cte_wp_ats)
+  apply (drule_tac p="(t, tcb_cnode_index 3)" in cte_wp_at_norm)
+  apply clarsimp
+  apply (drule pspace_relation_cte_wp_at[rotated])
+     apply (fastforce simp: valid_fault_handler_def has_handler_rights_def
+                            isValidFaultHandler_def is_cap_simps cte_wp_at'_def)+
+  done
 
 lemmas threadSet_ipcbuffer_trivial
     = threadSet_invs_trivial[where F="tcbIPCBuffer_update F'" for F',
                               simplified inQ_def, simplified]
-
-crunches setPriority, setMCPriority
-  for cap_to'[wp]: "ex_nonz_cap_to' a"
-  (simp: crunch_simps wp: hoare_drop_imps ignore: haskell_assert tcbEPFindIndex)
 
 lemma tc_caps_invs':
   "\<lbrace> invs' and sch_act_simple and
